SetSpectrum is done

current-formalism/Spectra/SetSpectrum.v
@@ -21,269 +21,400 @@
 Require Import Utf8_core.
 Require Import Omega.
 Require Import SetoidList.
-Require Import MSets.
-Require Import Pactole.Preliminary.
+Require Import SetoidDec.
+Require Import Pactole.Util.Preliminary.
+Require Export Pactole.Util.FSets.FSetInterface.
+Require Export Pactole.Util.FSets.FSetFacts.
 Require Import Pactole.Robots.
 Require Import Pactole.Configurations.
+Require Import Pactole.RobotInfo.
+Require Import Pactole.Spectra.Definition.
 
 
-Module Make (Location : DecidableType)
-            (N : Size)
-            (Names : Robots.Robots(N))
-            (Info : DecidableTypeWithApplication(Location))
-            (Config : Configuration(Location)(N)(Names)(Info)) <: Spectrum (Location)(N)(Names)(Info)(Config).
+Section SetConstruction.
 
+Context {loc : Type}.
+Context `{EqDec loc}.
 
-(** Definition of spectra as sets of locations. *)
-Module M := MSetWeakList.Make(Location).
-Module Mdec := Decide(M).
-Module MProp := EqProperties(M).
-Export Mdec.
+(* FIXME: remove once we have the implem in FSetList. *)
+Context {FS : @FSet loc _ _}.
+Context {FSSpec : @FSetSpecs loc _ _ FS}.
+(* Existing Instance multiplicity_compat.
+Existing Instance FMOps_WMap.
+Existing Instance MakeFMultisetsFacts. *)
 
+Ltac fsetdec := set_iff; tauto.
+
+(* 
+Lemma eq_refl_left : forall (e : loc) A (a b:A), (if equiv_dec e e then a else b) = a.
+Proof.
+intros e A a b.
+destruct (equiv_dec e e) as [| Hneq].
+- reflexivity.
+- now elim Hneq.
+Qed.
+ *)
+(* 
 Notation "m1  ≡  m2" := (M.eq m1 m2) (at level 70).
 Notation "m1  ⊆  m2" := (M.Subset m1 m2) (at level 70).
 Notation "m1  [=]  m2" := (M.eq m1 m2) (at level 70, only parsing).
 Notation "m1  [c=]  m2" := (M.Subset m1 m2) (at level 70, only parsing).
+ *)
 
 (** **  Building sets from lists  **)
 
-Definition set l := fold_left (fun acc x => M.add x acc) l M.empty.
+Definition make_set l := fold_left (fun acc x => add x acc) l empty.
 
-Lemma set_nil : set nil [=] M.empty.
+Lemma make_set_nil : make_set nil == empty.
 Proof. reflexivity. Qed.
 
-Lemma set_cons_aux : forall l x m,
-  List.fold_left (fun acc y => M.add y acc) (x :: l) m [=]
-  M.add x (List.fold_left (fun acc x => M.add x acc) l m).
+Lemma make_set_cons_aux : forall l x m,
+  List.fold_left (fun acc y => add y acc) (x :: l) m ==
+  add x (List.fold_left (fun acc x => add x acc) l m).
 Proof.
-intro l. induction l; intros x m.
+intro l. induction l as [| e l]; intros x s.
 + reflexivity.
-+ simpl. intro.
-  assert (Hf : Proper (M.eq ==> eq ==> M.eq) (fun acc y => M.add y acc)).
-  { clear. intros s1 s2 Hs x y Hxy. now rewrite Hxy, Hs. }
-  rewrite (@fold_left_start _ _ Logic.eq M.eq _ _ _ Hf l _ (M.add x (M.add a m))).
++ simpl fold_left.
+  assert (Hf : Proper (equiv ==> equiv ==> equiv) (fun acc y => add y acc)).
+  { clear x. intros s1 s2 Hs x y Hxy. now rewrite Hxy, Hs. }
+  rewrite (@fold_left_start _ _ equiv equiv _ _ _ Hf l _ (add x (add e s))).
   apply IHl. intro. fsetdec.
 Qed.
 
-Lemma set_cons : forall x l, set (x :: l) [=] M.add x (set l).
-Proof. intros x l y. unfold set. now rewrite set_cons_aux. Qed.
+Lemma make_set_cons : forall x l, make_set (x :: l) == add x (make_set l).
+Proof. intros x l. unfold make_set. now rewrite make_set_cons_aux. Qed.
 
-Lemma set_empty : forall l, set l [=] M.empty <-> l = nil.
+Lemma make_set_empty : forall l, make_set l == empty <-> l = nil.
 Proof.
-intro l. split; intro H.
-+ destruct l as [| x l]. reflexivity. rewrite set_cons in H.
-  specialize (H x). rewrite M.add_spec in H. elim (@M.empty_spec x). rewrite <- H. now left.
-+ subst l. apply set_nil.
+intro l. split; intro Hl.
++ destruct l as [| x l]. reflexivity. rewrite make_set_cons in Hl.
+  specialize (Hl x). rewrite add_spec, empty_spec in Hl. intuition.
++ subst l. apply make_set_nil.
 Qed.
 
-Lemma set_app : forall l l', set (l ++ l') [=] M.union (set l) (set l').
+Lemma make_set_app : forall l l', make_set (l ++ l') == union (make_set l) (make_set l').
 Proof.
-induction l as [| e l]; intros l'; simpl.
-+ intro. fsetdec. 
-+ do 2 rewrite set_cons. intro x. destruct (Location.eq_dec x e) as [Heq | Heq].
-  - rewrite Heq, M.add_spec, IHl. repeat rewrite M.union_spec. rewrite M.add_spec. tauto.
-  - rewrite M.add_spec, IHl; auto. repeat rewrite M.union_spec. rewrite M.add_spec; tauto.
+induction l as [| e l]; intros l'.
++ rewrite make_set_nil. simpl. intro. fsetdec.
++ simpl List.app. rewrite 2 make_set_cons, IHl. intro. fsetdec.
 Qed.
 
-Instance set_compat : Proper (PermutationA Location.eq ==> M.eq) set.
+Instance make_set_compat : Proper (PermutationA equiv ==> equiv) make_set.
 Proof.
 intro l1. induction l1 as [| x l1]; intros l2 Hperm.
 + apply (PermutationA_nil _) in Hperm. now subst.
 + assert (Hx := @PermutationA_InA_inside _ _ _ x _ _ Hperm).
   destruct Hx as [l1' [y [l2' [Hxy Heq]]]]. now left. subst l2.
-  intro z. rewrite set_app, M.union_spec. do 2 rewrite set_cons.
-  destruct (Location.eq_dec x z) as [Heq | Hneq].
-  - rewrite <- Heq, <- Hxy. repeat rewrite M.add_spec. intuition.
+  intro z. rewrite make_set_app, union_spec, 2 make_set_cons.
+  destruct (x =?= z) as [Heq | Hneq].
+  - rewrite Heq in *. rewrite <- Hxy. repeat rewrite add_spec. intuition.
   - rewrite <- (PermutationA_middle _), Hxy in Hperm. apply (PermutationA_cons_inv _) in Hperm.
-    repeat rewrite M.add_spec. rewrite (IHl1 _ Hperm). rewrite set_app, M.union_spec, <- Hxy. intuition.
+    repeat rewrite add_spec. rewrite (IHl1 _ Hperm). rewrite make_set_app, Hxy. fsetdec.
 Qed.
 
-Lemma set_PermutationA : forall x l,
-  exists l' n, ~InA Location.eq x l' /\ PermutationA Location.eq l (alls x n ++ l').
+Lemma make_set_PermutationA : forall x l,
+  exists l' n, ~InA equiv x l' /\ PermutationA equiv l (alls x n ++ l').
 Proof.
-intros x l. induction l.
+intros x l. induction l as [| e l].
 * exists nil, 0. split. now auto. simpl. reflexivity.
-* destruct IHl as [l' [n [Hin Hperm]]]. destruct (Location.eq_dec a x) as [Heq | Heq].
+* destruct IHl as [l' [n [Hin Hperm]]]. destruct (e =?= x) as [Heq | Heq].
   + exists l', (S n). split; trivial. simpl. apply PermutationA_cons; assumption.
-  + exists (a :: l'), n. split.
+  + exists (e :: l'), n. split.
     - intro Habs. inversion_clear Habs. elim Heq. now symmetry. contradiction.
     - rewrite Hperm. apply (PermutationA_middle _).
 Qed.
 
-Lemma set_alls : forall x n, 0 < n -> set (alls x n) [=] M.singleton x.
+Lemma make_set_alls : forall x n, 0 < n -> make_set (alls x n) == singleton x.
 Proof.
-intros x n Hn. induction n; simpl.
+intros x n Hn. induction n; simpl alls.
 + inversion Hn.
-+ rewrite set_cons. destruct n.
-  - simpl. rewrite set_nil. intro. fsetdec.
++ rewrite make_set_cons. destruct n.
+  - simpl alls. rewrite make_set_nil. intro. fsetdec.
   - rewrite IHn. intro. fsetdec. omega.
 Qed.
 
-Theorem set_spec : forall x l, M.In x (set l) <-> InA Location.eq x l.
+Theorem make_set_spec : forall x l, In x (make_set l) <-> InA equiv x l.
 Proof.
 intros x l. induction l.
-+ rewrite set_nil. intuition.
-+ rewrite set_cons, M.add_spec. intuition. inversion_clear H1; auto.
++ rewrite make_set_nil, InA_nil. fsetdec.
++ rewrite make_set_cons, add_spec, IHl. intuition. inversion_clear H2; auto.
 Qed.
 
-Theorem cardinal_set : forall l, M.cardinal (set l) <= length l.
+Theorem cardinal_make_set : forall l, cardinal (make_set l) <= length l.
 Proof.
 induction l as [| x l]; simpl.
-+ now rewrite set_nil.
-+ rewrite set_cons. destruct (M.mem x (set l)) eqn:Hmem.
-  - apply MProp.add_cardinal_1 in Hmem. omega.
-  - apply MProp.add_cardinal_2 in Hmem. omega.
++ now rewrite make_set_nil, cardinal_empty.
++ transitivity (S (cardinal (make_set l))); try omega; [].
+  rewrite make_set_cons, 2 cardinal_spec.
+  change (S (length (elements (make_set l))))
+    with (length (x :: elements (make_set l))).
+  apply NoDupA_inclA_length with equiv.
+  - autoclass.
+  - apply elements_NoDupA.
+  - apply elements_add_incl.
 Qed.
 
-Instance elements_compat : Proper (M.eq ==> PermutationA Location.eq) M.elements.
-Proof. repeat intro. apply NoDupA_equivlistA_PermutationA; autoclass; now apply M.elements_spec2w. Qed.
-
-
-(** Building a spectrum from a configuration *)
-
-(** Inclusion is not possible because M already contains a function [is_ok]. *)
-Definition t := M.t.
-Definition eq := M.eq.
-Definition eq_equiv := M.eq_equiv.
-Definition eq_dec := M.eq_dec.
-Definition In := M.In.
-
-Definition from_config conf : M.t := set (List.map Config.loc (Config.list conf)).
-
-Instance from_config_compat : Proper (Config.eq ==> M.eq) from_config.
+Theorem cardinal_NoDupA_make_set : forall l, NoDupA equiv l -> cardinal (make_set l) = length l.
 Proof.
-repeat intro. unfold from_config. do 2 f_equiv.
-apply (@PermutationA_map _ _ Config.eq_RobotConf Location.eq _ Config.loc).
-+ now intros ? ? [Heq _].
-+ apply eqlistA_PermutationA_subrelation, Config.list_compat. assumption.
+intros l Hl. induction l as [| x l]; simpl.
+- now rewrite make_set_nil, cardinal_empty.
+- inv Hl. rewrite <- IHl; trivial; [].
+  rewrite make_set_cons, cardinal_add; trivial; [].
+  now rewrite make_set_spec.
 Qed.
 
-Definition is_ok s conf := forall l,
-  In l s <-> exists id : Names.ident, Location.eq l (Config.loc (conf id)).
-
-Theorem from_config_spec : forall config, is_ok (from_config config) config.
+Instance fold_compat {A B} `{FSetSpecs A} `{Setoid B} :
+  forall f : A -> B -> B, Proper (equiv ==> equiv ==> equiv) f -> transpose equiv f ->
+  forall a, Proper (equiv ==> equiv) (fun x => fold f x a).
 Proof.
-unfold from_config, is_ok. intros config l.
-rewrite set_spec, InA_map_iff; autoclass.
-setoid_rewrite Config.list_InA. split.
-- intros [[pt info] [Heq [id Hid]]]. exists id. now rewrite <- Hid, <- Heq.
-- intros [id Hid]. exists (config id). intuition. now exists id.
-Qed.
-
-Definition map f m := M.fold (fun x acc => M.add (f x) acc) m M.empty.
-
-Instance fold_compat :
-    forall f, Proper (Location.eq ==> eq ==> eq) f -> transpose eq f ->
-    forall a, Proper (eq ==> eq) (fun x => M.fold f x a).
-Proof.
-intros f Hf Ht a m1 m2 Heq. do 2 rewrite M.fold_spec.
-rewrite fold_left_symmetry_PermutationA; autoclass; try reflexivity; [|].
+intros f Hf Ht a m1 m2 Heq. do 2 rewrite fold_spec.
+rewrite fold_left_symmetry_PermutationA; autoclass; [|].
 - repeat intro. now apply Hf.
-- apply NoDupA_equivlistA_PermutationA; autoclass; apply M.elements_spec2w.
+- now rewrite Heq.
 Qed.
-  
-Instance map_compat : forall f, Proper (Location.eq ==> Location.eq) f ->
-  Proper (eq ==> eq) (map f).
+
+Lemma fold_left_add_acc {A B} `{FSet A} `{FSetSpecs B} : forall (f : A -> B), Proper (equiv ==> equiv) f ->
+  forall x l acc, In x (fold_left (fun acc y => add (f y) acc) l acc)
+                  <-> In x acc \/ exists y, InA equiv y l /\ x == f y.
+Proof.
+intros f Hf x l. induction l as [| e l]; intro acc; simpl.
++ intuition.
+  match goal with H : exists _, InA _ _ nil /\ _ |- _ =>
+    destruct H as [? [H _]]; now rewrite InA_nil in H end.
++ rewrite IHl. set_iff. split; intro Hin.
+  - destruct Hin as [[? | ?] | [? [? ?]]]; try tauto; eauto.
+  - destruct Hin as [Heq | [? [Hin Heq]]]; tauto || inv Hin; eauto.
+    do 2 left. match goal with H : _ == e |- _ => now rewrite <- H end.
+Qed.
+
+(* Instance elements_compat : Proper (equiv ==> PermutationA equiv) elements := elements_compat. *)
+Definition map {A B} `{FSet A} `{FSet B} (f : A -> B) m :=
+  fold (fun x acc => add (f x) acc) m empty.
+
+Instance map_compat : forall f, Proper (equiv ==> equiv) f ->
+  Proper (equiv ==> equiv) (map f).
 Proof.
 intros f Hf m₁ m₂ Hm. unfold map. apply fold_compat; autoclass; [|].
 - repeat intro. now repeat f_equiv.
-- repeat intro. now rewrite MProp.MP.add_add.
+- repeat intro. fsetdec.
 Qed.
 
-Lemma map_empty : forall f, map f M.empty [=] M.empty.
+Lemma map_empty : forall f, map f empty == empty.
+Proof. intro. unfold map. rewrite fold_spec, elements_empty. simpl. reflexivity. Qed.
+
+(*
+Lemma fold_add_out {A B} `{FSetSpecs A} `{Setoid B} :
+  forall (f : A -> B -> B), Proper (equiv ==> equiv ==> equiv) f -> transpose2 equiv f ->
+  forall x m acc, ~In x m -> fold f (add x m) acc == fold f m (f x acc).
+Proof.
+intros f Hf Hf2 x m acc Hx.
+assert (Hf' : Proper (equiv ==> equiv ==> equiv) (fun x y => f y x)).
+{ repeat intro. now apply Hf. }
+assert (Hf2' : forall x y z, f y (f x z) == (f x (f y z))) by auto.
+assert (Hperm : PermutationA equiv (elements {x; m}) (x :: elements m)).
+{ apply NoDupA_equivlistA_PermutationA; autoclass.
+  + apply elements_NoDupA.
+  + constructor.
+    - now rewrite elements_spec.
+    - apply elements_NoDupA.
+  + intro y. rewrite elements_spec. set_iff.
+    split; intro Hin.
+    - intuition.
+    - inv Hin. now left. rewrite <- elements_spec; auto. }
+rewrite 2 fold_spec.
+rewrite (fold_left_symmetry_PermutationA _ _ Hf' Hf2');
+try apply Hperm; simpl; reflexivity.
+Qed.
+
+Lemma fold_add_in {A B} `{FSetSpecs A} `{Setoid B} :
+  forall (f : A -> B -> B), Proper (equiv ==> equiv ==> equiv) f -> transpose2 equiv f ->
+  forall x m acc, In x m -> fold f (add x m) acc == fold f m acc.
+Proof.
+intros f Hf Hf2 x m acc Hx.
+assert (Hf' : Proper (equiv ==> equiv ==> equiv) (fun x y => f y x)).
+{ repeat intro. now apply Hf. }
+assert (Hf2' : forall x y z, f y (f x z) == (f x (f y z))) by auto.
+assert (Hperm : PermutationA equiv (elements {x; m}) (elements m)).
+{ apply NoDupA_equivlistA_PermutationA; autoclass.
+  + apply elements_NoDupA.
+  + apply elements_NoDupA.
+  + intro y. rewrite 2 elements_spec. set_iff. intuition. rewrite <- In_eq_iff; eauto. }
+rewrite 2 fold_spec.
+rewrite (fold_left_symmetry_PermutationA _ _ Hf' Hf2');
+try apply Hperm; simpl; reflexivity.
+Qed.
+
+Lemma map_In {A B} `{FSetSpecs A} `{FSetSpecs B} : forall f : A -> B, Proper (equiv ==> equiv) f ->
+  forall x m, In x m -> In (f x) (map f m).
+Proof.
+intros f Hf x m Hin.
+unfold map. generalize empty.
+setoid_rewrite fold_spec. rewrite <- elements_spec in Hin.
+induction (elements m); intro acc.
++ now rewrite InA_nil in Hin.
++ inv Hin; simpl.
+  - match goal with H : _ == _ |- _ => rewrite H end.
+    rewrite fold_left_add_acc, add_spec; trivial; []. now do 2 left.
+  - now apply IHl.
+Qed.
+
+Lemma map_add {A B} `{FSetSpecs A} `{FSetSpecs B} : forall f : A -> B, Proper (equiv ==> equiv) f ->
+  forall x m, map f (add x m) == add (f x) (map f m).
+Proof.
+intros f Hf x m y.
+assert (Proper (equiv ==> equiv ==> equiv) (fun x acc => add (f x) acc)).
+{ intros ? ? Heq ? ? Heq' ?. rewrite Heq, Heq'. fsetdec. }
+assert (transpose2 equiv (fun x acc => add (f x) acc)).
+{ intros ? ? ? ? Heq ?. rewrite Heq. fsetdec. }
+destruct (mem x m) eqn:Hin.
++ rewrite mem_spec in Hin. unfold map at 1.
+  rewrite fold_add_in; autoclass; [].
+  change (fold (fun x acc => add (f x) acc) m empty) with (map f m).
+  set_iff. intuition.
+  match goal with H : _ == _ |- _ => rewrite <- H end.
+  now apply map_In.
++ rewrite mem_false in Hin. unfold map at 1.
+  rewrite fold_add_out, fold_spec, fold_left_add_acc; autoclass; [].
+  set_iff.
+  split; intro Hy.
+  - destruct Hy as [[|] | [? [Hy Heq]]]; try tauto; [].
+    right. rewrite Heq. rewrite elements_spec in Hy. now apply map_In.
+  - unfold map in Hy. rewrite fold_spec, fold_left_add_acc, empty_spec in Hy; trivial; [].
+    destruct Hy as [? | [? | [? [Hy Heq]]]]; eauto.
+Qed.
+*)
+
+Lemma map_spec {A B} `{FSetSpecs A} `{FSetSpecs B} : forall f : A -> B, Proper (equiv ==> equiv) f ->
+  forall y s, In y (map f s) <-> exists x, In x s /\ y == (f x).
+Proof.
+intros f Hf y s. unfold map.
+rewrite fold_spec, fold_left_add_acc, empty_spec; trivial; [].
+setoid_rewrite elements_spec. intuition.
+Qed.
+
+Corollary map_In {A B} `{FSetSpecs A} `{FSetSpecs B} : forall f : A -> B, Proper (equiv ==> equiv) f ->
+  forall x m, In x m -> In (f x) (map f m).
+Proof. repeat intro. rewrite map_spec; eauto. Qed.
+
+Corollary map_add {A B} `{FSetSpecs A} `{FSetSpecs B} : forall f : A -> B, Proper (equiv ==> equiv) f ->
+  forall x m, map f (add x m) == add (f x) (map f m).
+Proof.
+intros f Hf x m y. set_iff. rewrite 2 map_spec; trivial; [].
+split; intro Hin.
++ destruct Hin as [? [Hin Hy]]. revert Hin. set_iff. intros [Hx | Hin].
+  - rewrite Hy, Hx. now left.
+  - right. eauto.
++ destruct Hin as [Hy | [? [Hin Hx]]]; eexists; set_iff; eauto.
+Qed.
+
+Lemma map_injective_elements {A B} `{FSetSpecs A} `{FSetSpecs B} : forall f,
+  Proper (equiv ==> equiv) f ->
+  injective equiv equiv f ->
+  forall s, PermutationA equiv (elements (map f s)) (List.map f (elements s)).
+Proof.
+intros f Hf Hf2 s.
+apply NoDupA_equivlistA_PermutationA; autoclass.
++ apply elements_NoDupA.
++ eapply map_injective_NoDupA, elements_NoDupA; autoclass.
++ intro y.
+  rewrite elements_spec, map_spec, InA_map_iff; autoclass; [].
+  split; intros [x [Hx1 Hx2]].
+  - exists x. rewrite elements_spec. auto.
+  - exists x. rewrite <- elements_spec. now symmetry in Hx1.
+Qed.
+
+
+Theorem make_set_map : forall f, Proper (equiv ==> equiv) f ->
+  forall l, make_set (List.map f l) == map f (make_set l).
+Proof.
+intros f Hf l. induction l; simpl List.map.
++ now rewrite make_set_nil, map_empty.
++ do 2 rewrite make_set_cons. now rewrite map_add, IHl.
+Qed.
+
+End SetConstruction.
+
+(** Building a spectrum from a configuration *)
+
+Section SetSpectrum.
+
+Context {loc info : Type}.
+Context `{EqDec loc}.
+Context `{EqDec info}.
+Context {Loc : IsLocation loc info}.
+Context `{Names}.
+
+(* FIXME: remove once we have the implem in FSetList. *)
+Context {FS : @FSet loc _ _}.
+Context {FSSpec : @FSetSpecs loc _ _ FS}.
+
+Notation configuration := (@configuration info _ _ _ _).
+Notation map_config := (@map_config info _ _ _ _).
+Notation config_list := (@config_list info _ _ _ _).
+
+Implicit Type config : configuration.
+
+Global Instance set_spectrum : Spectrum loc info := {
+  spectrum := set loc;
+  
+  spect_from_config config pt := make_set (List.map get_location (config_list config));
+  spect_is_ok s config pt :=
+    forall l, In l s <-> InA equiv l (List.map get_location (config_list config)) }.
+Proof.
++ repeat intro.
+  apply make_set_compat, eqlistA_PermutationA_subrelation,
+        (@map_eqlistA_compat _ _ equiv equiv _ get_location).
+  - autoclass.
+  - apply config_list_compat. assumption.
++ unfold spect_from_config, spect_is_ok. intros. apply make_set_spec.
+Defined.
+
+Notation spectrum := (@spectrum loc info _ _ _ _ _ _ _).
+Notation spect_from_config := (@spect_from_config loc info _ _ _ _ _ _ set_spectrum).
+
+Require Pactole.Spaces.RealMetricSpace.
+Lemma spect_from_config_ignore_snd {RMS : RealMetricSpace.RealMetricSpace loc} : forall config pt,
+  spect_from_config config pt == spect_from_config config RealMetricSpace.origin.
 Proof. reflexivity. Qed.
 
-Lemma map_In : forall f, Proper (Location.eq ==> Location.eq) f ->
-  forall x m, M.In x m -> M.In (f x) (map f m).
+Lemma spect_from_config_map : forall f, Proper (equiv ==> equiv) f ->
+  forall config pt,
+  map f (spect_from_config config pt) == spect_from_config (map_config (app f) config) (f pt).
 Proof.
-intros f Hf x m.
-unfold map.
-apply MProp.MP.fold_rec_bis.
-+ intros s s' a Heq IH Hin.
-  apply IH.
-  now rewrite Heq.
-+ intro Hin.
-  apply MProp.MP.Dec.F.empty_iff in Hin.
-  elim Hin.
-+ intros a s s' Hina Hnotinta IH Hinx.
-  destruct (Location.eq_dec x a).
-  - rewrite e. now apply F.add_1.
-  - apply F.add_2.
-    apply IH.
-    apply F.add_3 with (x := a).
-    intro Heq. apply n. now rewrite Heq.
-    assumption.
+repeat intro. unfold spect_from_config, set_spectrum.
+rewrite config_list_map, map_map, <- make_set_map, map_map.
++ apply make_set_compat, Preliminary.eqlistA_PermutationA_subrelation.
+  assert (Hequiv : (equiv ==> equiv)%signature (fun x => f (get_location x)) (fun x => get_location (app f x))).
+  { intros pt1 pt2 Heq. now rewrite get_location_app, Heq. }
+  now apply (map_extensionalityA_compat _ Hequiv).
++ assumption.
++ now apply app_compat.
 Qed.
 
-Lemma map_add : forall f, Proper (Location.eq ==> Location.eq) f ->
-  forall x m, map f (M.add x m) [=] M.add (f x) (map f m).
+Theorem cardinal_spect_from_config : forall config pt, cardinal (spect_from_config config pt) <= nG + nB.
 Proof.
-  intros f Hf x m y.
-  destruct (MSetDecideAuxiliary.dec_In x m).
-  + unfold map at 1. rewrite MProp.MP.add_fold.
-    - assert (M.In (f x) (map f m)).
-      { now apply map_In. }
-      now rewrite MProp.MP.add_equal.
-    - apply eq_equiv.
-    - repeat intro. now rewrite H0, H1.
-    - repeat intro. now rewrite MProp.MP.add_add.
-    - assumption.
-  + unfold map at 1. rewrite MProp.MP.fold_add.
-    - reflexivity.
-    - apply eq_equiv.
-    - repeat intro. now rewrite H0, H1.
-    - repeat intro. now rewrite MProp.MP.add_add.
-    - assumption.
+intros. unfold spect_from_config, set_spectrum.
+etransitivity; try apply cardinal_make_set; [].
+now rewrite map_length, config_list_length.
 Qed.
 
-Lemma map_spec : forall f, Proper (Location.eq ==> Location.eq) f ->
-  forall y s, M.In y (map f s) <-> exists x, M.In x s /\ Location.eq y (f x).
+Property pos_in_config : forall config pt id, In (get_location (config id)) (spect_from_config config pt).
 Proof.
-intros f Hf y s. split.
-* pattern s. apply MProp.set_rec; clear s.
-  + intros s s' Heq Hrec Hin. rewrite <- F.equal_iff in Heq.
-    rewrite <- Heq in Hin. apply Hrec in Hin. setoid_rewrite <- Heq. apply Hin.
-  + intros s x Hout Hrec Hin. rewrite map_add in Hin; autoclass.
-    rewrite M.add_spec in Hin. destruct Hin as [Hin | Hin].
-    - exists x. fsetdec.
-    - apply Hrec in Hin. destruct Hin as [x' [Hin Heq]].
-      exists x'. fsetdec.
-  + intro. fsetdec.
-* intros [x [Hin Heq]]. rewrite Heq. now apply map_In.
+intros config pt id. unfold spect_from_config. simpl.
+rewrite make_set_spec, InA_map_iff; autoclass; [].
+eexists. split; auto; []. apply config_list_InA. now exists id.
 Qed.
 
-Theorem set_map : forall f, Proper (Location.eq ==> Location.eq) f ->
-  forall l, set (List.map f l) [=] map f (set l).
+Property spect_from_config_In : forall config pt l,
+  In l (spect_from_config config pt) <-> exists id, get_location (config id) == l.
 Proof.
-intros f Hf l.
-induction l; simpl.
-+ now rewrite set_nil, map_empty.
-+ do 2 rewrite set_cons. now rewrite map_add, IHl.
+intros config pt l. split; intro Hin.
++ assert (Heq := spect_from_config_spec config pt).
+  unfold spect_is_ok, spect_from_config, set_spectrum in *.
+  rewrite Heq, config_list_spec, map_map, (InA_map_iff _ _) in Hin.
+  - firstorder.
+  - repeat intro. cbn in *. now subst.
++ destruct Hin as [id Hid]. rewrite <- Hid. apply pos_in_config.
 Qed.
 
-
-Lemma from_config_map : forall f, Proper (Location.eq ==> Location.eq) f ->
-  forall config, eq (map f (from_config config)) (from_config (Config.map (Config.app f) config)).
-Proof.
-intros f Hf config. unfold from_config.
-rewrite Config.list_map, <- set_map; autoclass.
-do 2 rewrite List.map_map. f_equiv.
-Qed.
-
-Lemma map_injective_elements : forall f,
-  Proper (Location.eq ==> Location.eq) f ->
-  injective Location.eq Location.eq f ->
-  forall s, PermutationA Location.eq (M.elements (map f s)) (List.map f (M.elements s)).
-Proof.
-intros f Hf Hfinj s.
-apply NoDupA_equivlistA_PermutationA; autoclass.
-+ apply M.elements_spec2w.
-+ eapply map_injective_NoDupA; autoclass. apply M.elements_spec2w.
-+ intro y.
-  rewrite <- F.elements_iff, map_spec, InA_map_iff; autoclass; [].
-  split; intros [x [H1 H2]].
-  - exists x. fsetdec.
-  - exists x. rewrite MProp.MP.Dec.F.elements_iff. now symmetry in H1.
-Qed.
-
-End Make.
+End SetSpectrum.
