current-formalism/Util/FSets/FSetFacts.v
@@ -1,12 +1,15 @@
 (* Order of import is important here, Equivalence.equiv must be hidden by SetoidClass.equiv. *)
-Require Import Coq.Classes.Equivalence Morphisms SetoidList SetoidDec Program.Basics.
-Require Import Pactole.Util.FSets.FsetInterface.
+Require Import Coq.Classes.Equivalence Morphisms.
+Require Import SetoidList SetoidPermutation SetoidDec.
+Require Import Program.Basics.
+Require Import Pactole.Util.FSets.FSetInterface.
 Set Implicit Arguments.
 Unset Strict Implicit.
 
 Generalizable All Variables.
 Local Open Scope set_scope.
 Local Open Scope equiv_scope.
+
 
 (** This file corresponds to [FSetFacts.v] in the standard library.
    There are additional specifications, for boolean functions in particular,
@@ -23,7 +26,7 @@ Notation Leibniz := (@eq _) (only parsing).
 Section IffSpec.
   Context `{HF : @FSetSpecs elt St Helt F}.
 
-  Let t := set.
+  Let t := set elt.
   Definition eq_b x y := x == y.
   Variable s s' s'' : t.
   Variable x y z : elt.
@@ -33,57 +36,43 @@ Section IffSpec.
     split; apply In_1;intros; auto.
   Qed.
 
-  Lemma mem_iff : In x s <-> mem x s = true.
+  Lemma mem_spec : mem x s = true <-> In x s.
+  Proof. split; [apply mem_2 | apply mem_1]. Qed.
+
+  Lemma mem_false : mem x s = false <-> ~In x s.
+  Proof. intros; rewrite <- mem_spec; destruct (mem x s); intuition. Qed.
+
+  Lemma equal_spec : equal s s' = true <-> s == s'.
+  Proof. split; [apply equal_2 | apply equal_1]. Qed.
+
+  Lemma subset_spec : subset s s' = true <-> s [<=] s'.
+  Proof. split; [apply subset_2 | apply subset_1]. Qed.
+
+  Lemma empty_spec : forall x, In x empty <-> False.
+  Proof. intuition; apply (empty_1 H). Qed.
+
+  Lemma is_empty_spec : is_empty s = true <-> s == empty.
   Proof.
-    split; [apply mem_1|apply mem_2].
+  split.
+  - intros H e. apply is_empty_2 in H. specialize (H e). rewrite empty_spec. tauto.
+  - intro Heq. apply is_empty_1. intro e. rewrite (Heq e), empty_spec. tauto.
   Qed.
 
-  Lemma not_mem_iff : ~In x s <-> mem x s = false.
-  Proof.
-    intros; rewrite mem_iff; destruct (mem x s); intuition.
-  Qed.
+  Lemma singleton_spec : In y (singleton x) <-> x == y.
+  Proof. split; [apply singleton_1|apply singleton_2]. Qed.
 
-  Lemma equal_iff : s[=]s' <-> equal s s' = true.
+  Lemma add_spec : In y (add x s) <-> x == y \/ In y s.
   Proof.
-    split; [apply equal_1|apply equal_2].
-  Qed.
-
-  Lemma subset_iff : s[<=]s' <-> subset s s' = true.
-  Proof.
-    split; [apply subset_1|apply subset_2].
-  Qed.
-
-  Lemma empty_iff : In x empty <-> False.
-  Proof.
-    intuition; apply (empty_1 H).
-  Qed.
-
-  Lemma is_empty_iff : Empty s <-> is_empty s = true.
-  Proof.
-    split; [apply is_empty_1|apply is_empty_2].
-  Qed.
-
-  Lemma singleton_iff : In y (singleton x) <-> x == y.
-  Proof.
-    split; [apply singleton_1|apply singleton_2].
-  Qed.
-
-  Lemma add_iff : In y (add x s) <-> x == y \/ In y s.
-  Proof.
-    split; [ | destruct 1; [apply add_1|apply add_2]]; auto.
+    split; [| destruct 1; [apply add_1 | apply add_2]]; auto.
     destruct (Helt x y) as [E|E].
-    - intro.
-      auto.
-    - intro H; right.
-      exact (add_3 E H).
+    - intro. auto.
+    - intro H; right. eauto using add_3.
   Qed.
 
-  Lemma add_neq_iff : x =/= y -> (In y (add x s)  <-> In y s).
-  Proof.
-    split; [apply add_3|apply add_2]; auto.
-  Qed.
+  Lemma add_other : x =/= y -> (In y (add x s) <-> In y s).
+  Proof. split; [apply add_3 | apply add_2]; auto. Qed.
 
-  Lemma remove_iff : In y (remove x s) <-> In y s /\ x =/= y.
+  Lemma remove_spec : In y (remove x s) <-> In y s /\ x =/= y.
   Proof.
     split; [split;
       [apply remove_3 with x |] | destruct 1; apply remove_2]; auto.
@@ -91,33 +80,32 @@ Section IffSpec.
     apply (remove_1 H0 H).
   Qed.
 
-  Lemma remove_neq_iff : x =/= y -> (In y (remove x s) <-> In y s).
-  Proof.
-    split; [apply remove_3|apply remove_2]; auto.
-  Qed.
+  Lemma remove_other : x =/= y -> (In y (remove x s) <-> In y s).
+  Proof. split; [apply remove_3 | apply remove_2]; auto. Qed.
 
-  Lemma union_iff : In x (union s s') <-> In x s \/ In x s'.
-  Proof.
-    split; [apply union_1 | destruct 1; [apply union_2|apply union_3]]; auto.
-  Qed.
+  Lemma union_spec : In x (union s s') <-> In x s \/ In x s'.
+  Proof. split; [apply union_1 | destruct 1; [apply union_2 | apply union_3]]; auto. Qed.
 
-  Lemma inter_iff : In x (inter s s') <-> In x s /\ In x s'.
+  Lemma inter_spec : In x (inter s s') <-> In x s /\ In x s'.
   Proof.
     split; [split; [apply inter_1 with s' |
       apply inter_2 with s] | destruct 1; apply inter_3]; auto.
   Qed.
 
-  Lemma diff_iff : In x (diff s s') <-> In x s /\ ~ In x s'.
+  Lemma diff_spec : In x (diff s s') <-> In x s /\ ~ In x s'.
   Proof.
     split; [split; [apply diff_1 with s' |
       apply diff_2 with s] | destruct 1; apply diff_3]; auto.
   Qed.
 
+  Lemma elements_spec : InA equiv x (elements s) <-> In x s.
+  Proof. split; [apply elements_2 | apply elements_1]. Qed.
+
   Section ForFilter.
     Variable f : elt -> bool.
     Context {Hf : Proper (equiv ==> @eq bool) f}.
 
-    Lemma filter_iff : (In x (filter f s) <-> In x s /\ f x = true).
+    Lemma filter_spec : (In x (filter f s) <-> In x s /\ f x = true).
     Proof.
       split.
       - split.
@@ -126,57 +114,48 @@ Section IffSpec.
       - destruct 1; eapply filter_3; eauto.
     Qed.
 
-    Lemma for_all_iff :
-      (For_all (fun x => f x = true) s <-> for_all f s = true).
-    Proof.
-      split; [eapply for_all_1;eauto | eapply for_all_2;eauto]; auto.
-    Qed.
+    Lemma for_all_spec : for_all f s = true <-> For_all (fun x => f x = true) s.
+    Proof. split; [eapply for_all_2; eauto | eapply for_all_1; eauto]; auto. Qed.
 
-    Lemma exists_iff : (Exists (fun x => f x = true) s <-> exists_ f s = true).
-    Proof.
-      split; [eapply exists_1 | eapply exists_2]; eauto.
-    Qed.
+    Lemma exists_spec : exists_ f s = true <-> Exists (fun x => f x = true) s.
+    Proof. split; [eapply exists_2 | eapply exists_1]; eauto. Qed.
   End ForFilter.
   Arguments InA {A%type_scope} _ _ _.
-  Lemma elements_iff : In x s <-> InA equiv x (elements s).
-  Proof.
-    split; [apply elements_1 | apply elements_2].
-  Qed.
 
 End IffSpec.
 
 (** Useful tactic for simplifying expressions like [In y (add x (union s s'))]*)
 Ltac set_iff :=
  repeat (progress (
-  rewrite add_iff || rewrite remove_iff || rewrite singleton_iff
-  || rewrite union_iff || rewrite inter_iff || rewrite diff_iff
-  || rewrite empty_iff)).
+  rewrite add_spec || rewrite remove_spec || rewrite singleton_spec
+  || rewrite union_spec || rewrite inter_spec || rewrite diff_spec
+  || rewrite empty_spec)).
 
 (**  * Specifications written using boolean predicates *)
 Require Import Bool.
 Section BoolSpec.
   Context `{HF : @FSetSpecs elt St Helt F}.
 
-  Let t := set.
+  Let t := set elt.
   Variable s s' s'' : t.
   Variable x y z : elt.
 
   Lemma mem_b : x == y -> mem x s = mem y s.
   Proof.
     intros.
-    generalize (mem_iff s x) (mem_iff s y) (In_eq_iff s H).
+    generalize (mem_spec s x) (mem_spec s y) (In_eq_iff s H).
     destruct (mem x s); destruct (mem y s); intuition.
   Qed.
 
   Lemma empty_b : mem y empty = false.
   Proof.
-    generalize (empty_iff y)(mem_iff empty y).
+    generalize (empty_spec y)(mem_spec empty y).
     destruct (mem y empty); intuition.
   Qed.
 
   Lemma add_b : mem y (add x s) = (x ==b y) || mem y s.
   Proof.
-    generalize (mem_iff (add x s) y)(mem_iff s y)(add_iff s x y); unfold eqb.
+    generalize (mem_spec (add x s) y)(mem_spec s y)(add_spec s x y); unfold eqb.
     unfold equiv_decb.
     destruct (equiv_dec x y) ; destruct (mem y s);
       destruct (mem y (add x s)); simpl;intuition.
@@ -184,69 +163,68 @@ Section BoolSpec.
 
   Lemma add_neq_b : x =/= y -> mem y (add x s) = mem y s.
   Proof.
-    intros; generalize (mem_iff (add x s) y)(mem_iff s y)(add_neq_iff s H).
+    intros; generalize (mem_spec (add x s) y)(mem_spec s y)(add_other s H).
     destruct (mem y s); destruct (mem y (add x s)); intuition.
   Qed.
 
   Lemma remove_b : mem y (remove x s) = mem y s && negb (x ==b y).
   Proof.
-    generalize (mem_iff (remove x s) y)(mem_iff s y)(remove_iff s x y).
+    generalize (mem_spec (remove x s) y)(mem_spec s y)(remove_spec s x y).
     unfold equiv_decb;destruct (equiv_dec x y); destruct (mem y s); destruct (mem y (remove x s));
       simpl; intuition ; contradiction.
   Qed.
 
   Lemma remove_neq_b : x =/= y -> mem y (remove x s) = mem y s.
   Proof.
-    intros; generalize (mem_iff (remove x s) y) (mem_iff s y)
-      (remove_neq_iff s H).
+    intros; generalize (mem_spec (remove x s) y) (mem_spec s y)
+      (remove_other s H).
     destruct (mem y s); destruct (mem y (remove x s)); intuition.
   Qed.
 
   Lemma singleton_b : mem y (singleton x) = (x ==b y).
   Proof.
-    generalize (mem_iff (singleton x) y)(singleton_iff x y); unfold eqb.
+    generalize (mem_spec (singleton x) y)(singleton_spec x y); unfold eqb.
     unfold equiv_decb;destruct (equiv_dec x y); destruct (mem y (singleton x)); intuition.
   Qed.
 
   Lemma union_b : mem x (union s s') = mem x s || mem x s'.
   Proof.
-    generalize (mem_iff (union s s') x)(mem_iff s x)(mem_iff s' x)
-      (union_iff s s' x).
+    generalize (mem_spec (union s s') x)(mem_spec s x)(mem_spec s' x)
+      (union_spec s s' x).
     destruct (mem x s); destruct (mem x s');
       destruct (mem x (union s s')); intuition.
   Qed.
 
   Lemma inter_b : mem x (inter s s') = mem x s && mem x s'.
   Proof.
-    generalize (mem_iff (inter s s') x)(mem_iff s x)
-      (mem_iff s' x)(inter_iff s s' x).
+    generalize (mem_spec (inter s s') x)(mem_spec s x)
+      (mem_spec s' x)(inter_spec s s' x).
     destruct (mem x s); destruct (mem x s');
       destruct (mem x (inter s s')); intuition.
   Qed.
 
   Lemma diff_b : mem x (diff s s') = mem x s && negb (mem x s').
   Proof.
-    generalize (mem_iff (diff s s') x)(mem_iff s x)
-      (mem_iff s' x)(diff_iff s s' x).
+    generalize (mem_spec (diff s s') x)(mem_spec s x)
+      (mem_spec s' x)(diff_spec s s' x).
     destruct (mem x s); destruct (mem x s');
       destruct (mem x (diff s s')); simpl; intuition.
   Qed.
 
   Lemma elements_b : mem x s = existsb (fun y => x ==b y) (elements s).
   Proof.
-    generalize (mem_iff s x)(elements_iff s x)
+    generalize (mem_spec s x)(elements_spec s x)
       (existsb_exists (fun y => x ==b y) (elements s)).
     rewrite InA_alt.
     destruct (mem x s); destruct (existsb (fun y => x ==b y)
       (elements s)); auto; intros.
     symmetry.
     rewrite H1.
-    destruct H0 as (H0,_).
+    destruct H0 as (_, H0).
     destruct H0 as (a,(Ha1,Ha2)); [ intuition |].
     exists a; intuition.
     unfold equiv_decb; destruct (equiv_dec x a); auto.
-    rewrite <- H.
-    rewrite H0.
+    rewrite H, <- H0.
     destruct H1 as (H1,_).
     destruct H1 as (a,(Ha1,Ha2)); [intuition|].
     exists a; intuition.
@@ -259,7 +237,7 @@ Section BoolSpec.
     mem x (filter f s) = mem x s && f x.
   Proof.
     intros.
-    generalize (mem_iff (filter f s) x)(mem_iff s x)(filter_iff (f:=f) s x).
+    generalize (mem_spec (filter f s) x)(mem_spec s x)(filter_spec (f:=f) s x).
     destruct (mem x s); destruct (mem x (filter f s));
       destruct (f x); simpl; intuition.
   Qed.
@@ -269,21 +247,21 @@ Section BoolSpec.
   Proof.
     intros.
     generalize (forallb_forall f (elements s))
-      (for_all_iff (f:=f) s)(elements_iff s).
+      (for_all_spec (f:=f) s)(elements_spec s).
     unfold For_all.
     destruct (forallb f (elements s)); destruct (for_all f s); auto; intros.
-    rewrite <- H1; intros.
-    destruct H0 as (H0,_).
-    rewrite (H2 x0) in H3.
+    rewrite H1; intros.
+    destruct H0 as (H0, _).
+    rewrite <- (H2 x0) in H3.
     rewrite (InA_alt equiv x0 (elements s)) in H3.
     destruct H3 as (a,(Ha1,Ha2)).
     rewrite (H _ _ Ha1).
     apply H0; auto.
     symmetry.
     rewrite H0; intros.
-    destruct H1 as (_,H1).
+    destruct H1 as (H1, _).
     apply H1; auto.
-    rewrite H2.
+    rewrite <- H2.
     rewrite InA_alt; eauto.
   Qed.
 
@@ -292,19 +270,19 @@ Section BoolSpec.
   Proof.
     intros.
     generalize (existsb_exists f (elements s))
-      (exists_iff (f:=f) s)(elements_iff s).
+      (exists_spec (f:=f) s)(elements_spec s).
     unfold Exists.
     destruct (existsb f (elements s)); destruct (exists_ f s); auto; intros.
-    rewrite <- H1; intros.
+    rewrite H1; intros.
     destruct H0 as (H0,_).
     destruct H0 as (a,(Ha1,Ha2)); auto.
     exists a; split; auto.
-    rewrite H2; rewrite InA_alt; eauto.
+    rewrite <- H2; rewrite InA_alt; eauto.
     symmetry.
     rewrite H0.
-    destruct H1 as (_,H1).
+    destruct H1 as (H1, _).
     destruct H1 as (a,(Ha1,Ha2)); auto.
-    rewrite (H2 a) in Ha1.
+    rewrite <- (H2 a) in Ha1.
     rewrite (InA_alt equiv a (elements s)) in Ha1.
     destruct Ha1 as (b,(Hb1,Hb2)).
     exists b; auto.
@@ -312,124 +290,121 @@ Section BoolSpec.
   Qed.
 End BoolSpec.
 
-(** * [Equal] is a setoid equality *)
-Instance Equal_ST `{FSet A} : Equivalence Equal.
-Proof.
-  constructor; red ; intros.
-  intro e; tauto.
-  intro e; rewrite (H1 e); tauto.
-  intro e; transitivity (e \In y); [apply H1 | apply H2].
-Qed.
 
 Instance In_m `{HF : @FSetSpecs A St HA F} :
-  Proper (equiv ==> Equal ==> iff) In.
+  Proper (equiv ==> equiv ==> iff) In.
 Proof.
-  unfold Equal; intros x y H s s' H0.
+  intros x y H s s' H0.
   rewrite (In_eq_iff s H); auto.
 Qed.
 
 Instance is_empty_m `{HF : @FSetSpecs A St HA F} :
-  Proper (Equal ==> @eq bool)  is_empty.
+  Proper (equiv ==> @eq bool)  is_empty.
 Proof.
-  unfold Equal; intros s s' H.
-  generalize (is_empty_iff s)(is_empty_iff s').
+  intros s s' H.
+  generalize (is_empty_spec s)(is_empty_spec s').
   destruct (is_empty s); destruct (is_empty s');
-    unfold Empty; auto; intros.
-  symmetry.
-  rewrite <- H1; intros a Ha.
-  rewrite <- (H a) in Ha.
-  destruct H0 as (_,H0).
-  exact (H0 (refl_equal true) _ Ha).
-  rewrite <- H0; intros a Ha.
-  rewrite (H a) in Ha.
-  destruct H1 as (_,H1).
-  exact (H1 (refl_equal true) _ Ha).
+  unfold Empty; auto; intros.
+  - symmetry. now rewrite H1, <- H, <- H0.
+  - now rewrite H0, H, <- H1.
 Qed.
 
-Instance Empty_m `{HF : @FSetSpecs A St HA F} :
-  Proper (Equal ==> iff) Empty.
-Proof.
-  intros s s' H; do 2 rewrite is_empty_iff; rewrite H; intuition.
-Qed.
+Instance Empty_m `{HF : @FSetSpecs A St HA F} : Proper (equiv ==> iff) Empty.
+Proof. unfold Empty. intros ? ? H. now setoid_rewrite H. Qed.
 
 Instance mem_m `{HF : @FSetSpecs A St HA F} :
-  Proper (equiv ==> Equal ==> @eq bool) mem.
+  Proper (equiv ==> equiv ==> @eq bool) mem.
 Proof.
-  unfold Equal; intros x y H s s' H0.
+  intros x y H s s' H0.
   generalize (H0 x); clear H0; rewrite (In_eq_iff s' H).
-  generalize (mem_iff s x)(mem_iff s' y).
+  generalize (mem_spec s x)(mem_spec s' y).
   destruct (mem x s); destruct (mem y s'); intuition.
 Qed.
 
 Instance singleton_m `{HF : @FSetSpecs A St HA F} :
-  Proper (equiv ==> Equal) singleton.
+  Proper (equiv ==> equiv) singleton.
 Proof.
-  unfold Equal; intros x y H a.
-  do 2 rewrite singleton_iff.
+  intros x y H a.
+  do 2 rewrite singleton_spec.
   split; intros.
   - transitivity x; auto.
   - transitivity y; auto.
-  
 Qed.
 
 Instance add_m `{HF : @FSetSpecs A St HA F} :
-  Proper (equiv ==> Equal ==> Equal) add.
+  Proper (equiv ==> equiv ==> equiv) add.
 Proof.
-  unfold Equal; intros x y H s s' H0 a.
-  do 2 rewrite add_iff; rewrite H; rewrite H0; intuition.
+  intros x y H s s' H0 a.
+  do 2 rewrite add_spec; rewrite H; rewrite H0; intuition.
 Qed.
 
 Instance remove_m `{HF : @FSetSpecs A St HA F} :
-  Proper (equiv ==> Equal ==> Equal) remove.
+  Proper (equiv ==> equiv ==> equiv) remove.
 Proof.
-  unfold Equal; intros x y H s s' H0 a.
-  do 2 rewrite remove_iff; rewrite H; rewrite H0; intuition.
+  intros x y H s s' H0 a.
+  do 2 rewrite remove_spec; rewrite H; rewrite H0; intuition.
 Qed.
 
 Instance union_m `{HF : @FSetSpecs A St HA F} :
-  Proper (Equal ==> Equal ==> Equal) union.
+  Proper (equiv ==> equiv ==> equiv) union.
 Proof.
-  unfold Equal; intros s s' H s'' s''' H0 a.
-  do 2 rewrite union_iff; rewrite H; rewrite H0; intuition.
+  intros s s' H s'' s''' H0 a.
+  do 2 rewrite union_spec; rewrite H; rewrite H0; intuition.
 Qed.
 
 Instance inter_m `{HF : @FSetSpecs A St HA F} :
-  Proper (Equal ==> Equal ==> Equal) inter.
+  Proper (equiv ==> equiv ==> equiv) inter.
 Proof.
-  unfold Equal; intros s s' H s'' s''' H0 a.
-  do 2 rewrite inter_iff; rewrite H; rewrite H0; intuition.
+  intros s s' H s'' s''' H0 a.
+  do 2 rewrite inter_spec; rewrite H; rewrite H0; intuition.
 Qed.
 
 Instance diff_m `{HF : @FSetSpecs A St HA F} :
-  Proper (Equal ==> Equal ==> Equal) diff.
+  Proper (equiv ==> equiv ==> equiv) diff.
 Proof.
-  unfold Equal; intros s s' H s'' s''' H0 a.
-  do 2 rewrite diff_iff; rewrite H; rewrite H0; intuition.
+  intros s s' H s'' s''' H0 a.
+  do 2 rewrite diff_spec; rewrite H; rewrite H0; intuition.
 Qed.
 
-Instance Subset_m `{HF : @FSetSpecs A St HA F} :
-  Proper (Equal ==> Equal ==> iff) Subset.
+Instance elements_compat `{HF : @FSetSpecs A St HA F} :
+  Proper (equiv ==> PermutationA equiv) elements.
 Proof.
-  unfold Equal, Subset; intros s s' H u u' H'; split; intros.
+intros s s' Heq. apply NoDupA_equivlistA_PermutationA.
++ auto with typeclass_instances.
++ apply elements_NoDupA.
++ apply elements_NoDupA.
++ intro x. rewrite 2 elements_spec. apply Heq.
+Qed.
+
+Instance PermutationA_length {elt} `{Setoid elt} : Proper (PermutationA equiv ==> Logic.eq) (@length elt).
+Proof. clear. intros l1 l2 perm. induction perm; simpl; auto; congruence. Qed.
+
+Instance cardinal_compat `{HF : @FSetSpecs A St HA F} : Proper (equiv ==> Logic.eq) cardinal.
+Proof. intros ? ? Heq. rewrite 2 cardinal_spec. now do 2 f_equiv. Qed.
+
+Instance Subset_m `{HF : @FSetSpecs A St HA F} :
+  Proper (equiv ==> equiv ==> iff) Subset.
+Proof.
+  unfold Subset; intros s s' H u u' H'; split; intros.
   rewrite <- H'; apply H0; rewrite H; assumption.
   rewrite H'; apply H0; rewrite <- H; assumption.
 Qed.
 
 Instance subset_m `{HF : @FSetSpecs A St HA F} :
-  Proper (Equal ==> Equal ==> @eq bool) subset.
+  Proper (equiv ==> equiv ==> @eq bool) subset.
 Proof.
   intros s s' H s'' s''' H0.
-  generalize (subset_iff s s'') (subset_iff s' s''').
+  generalize (subset_spec s s'') (subset_spec s' s''').
   destruct (subset s s''); destruct (subset s' s'''); auto; intros.
   rewrite H in H1; rewrite H0 in H1; intuition.
   rewrite H in H1; rewrite H0 in H1; intuition.
 Qed.
 
 Instance equal_m `{HF : @FSetSpecs A St HA F} :
-  Proper (Equal ==> Equal ==> @eq bool) equal.
+  Proper (equiv ==> equiv ==> @eq bool) equal.
 Proof.
   intros s s' H s'' s''' H0.
-  generalize (equal_iff s s'') (equal_iff s' s''').
+  generalize (equal_spec s s'') (equal_spec s' s''').
   destruct (equal s s''); destruct (equal s' s'''); auto; intros.
   rewrite H in H1; rewrite H0 in H1; intuition.
   rewrite H in H1; rewrite H0 in H1; intuition.
@@ -468,52 +443,52 @@ Instance add_s_m `{F : FSet A, @FSetSpecs _ _ _ F} :
   Proper (equiv ==> Subset ++> Subset) add.
 Proof.
   unfold Subset; intros x y H1 s s' H2 a.
-  do 2 rewrite add_iff; rewrite H1; intuition.
+  do 2 rewrite add_spec; rewrite H1; intuition.
 Qed.
 
 Instance remove_s_m `{F : FSet A, @FSetSpecs _ _ _ F} :
   Proper (equiv ==> Subset ++> Subset) remove.
 Proof.
   unfold Subset; intros x y H1 s s' H2 a.
-  do 2 rewrite remove_iff; rewrite H1; intuition.
+  do 2 rewrite remove_spec; rewrite H1; intuition.
 Qed.
 
-Instance union_s_m `{@FSetSpecs _ _ _  F} :
+Instance union_s_m `{F : FSet A, @FSetSpecs _ _ _  F} :
   Proper (Subset ++> Subset ++> Subset) union.
 Proof.
-  unfold Equal; intros s s' H1 s'' s''' H2 a.
-  do 2 rewrite union_iff; intuition.
+  intros s s' H1 s'' s''' H2 a.
+  do 2 rewrite union_spec; intuition.
 Qed.
 
-Instance inter_s_m `{@FSetSpecs A St HA F} :
+Instance inter_s_m `{F : FSet A, @FSetSpecs _ _ _ F} :
   Proper (Subset ++> Subset ++> Subset) inter.
 Proof.
-  unfold Equal; intros s s' H1 s'' s''' H2 a.
-  do 2 rewrite inter_iff; intuition.
+  intros s s' H1 s'' s''' H2 a.
+  do 2 rewrite inter_spec; intuition.
 Qed.
 
-Instance diff_s_m `{@FSetSpecs A St HA F} :
+Instance diff_s_m `{F : FSet A, @FSetSpecs _ _ _ F} :
   Proper (Subset ++> Subset --> Subset) diff.
 Proof.
   unfold Subset; intros s s' H1 s'' s''' H2 a.
-  do 2 rewrite diff_iff; intuition.
+  do 2 rewrite diff_spec; intuition.
 Qed.
 
 (** [fold], [filter], [for_all], [exists_] and [partition] require
    the  additional hypothesis on [f]. *)
 Instance filter_m  `{F : FSet A, @FSetSpecs _ _ _ F} :
   forall f `{Proper _ (equiv ==> @eq bool) f},
-    Proper (Equal ==> Equal) (filter f).
+    Proper (equiv ==> equiv) (filter f).
 Proof.
-  unfold Equal; intros f Hf s s' H' x.
-  repeat rewrite filter_iff; auto. rewrite H'; reflexivity.
+  intros f Hf s s' H' x.
+  repeat rewrite filter_spec; auto. rewrite H'; reflexivity.
 Qed.
 
 Lemma filter_ext  `{F : FSet A, @FSetSpecs _ _ _ F} :
   forall f f' `{Proper _ (equiv ==> @eq bool) f}, (forall x, f x = f' x) ->
-    forall s s', s[=]s' -> filter f s [=] filter f' s'.
+    forall s s', s==s' -> filter f s == filter f' s'.
 Proof.
-  intros f f' Hf Hff' s s' Hss' x. do 2 (rewrite filter_iff; auto).
+  intros f f' Hf Hff' s s' Hss' x. do 2 (rewrite filter_spec; auto).
   rewrite Hff', Hss'; intuition.
   red; repeat intro; rewrite <- 2 Hff'; auto.
 Qed.
@@ -523,7 +498,7 @@ Instance filter_s_m  `{F : FSet A, @FSetSpecs _ _ _ F} :
     Proper (Subset ==> Subset) (filter f).
 Proof.
   unfold Subset; intros f Hf s s' H' x.
-  repeat rewrite filter_iff; auto; intro; intuition.
+  repeat rewrite filter_spec; auto; intro; intuition.
 Qed.
 
 (** * Inductive specifications of boolean functions *)
@@ -533,7 +508,7 @@ CoInductive reflects (P : Prop) : bool -> Prop :=
 
 Section InductiveSpec.
   Context `{HF : @FSetSpecs elt St Helt F}.
-  Variables s s' s'' : set.
+  Variables s s' s'' : set elt.
   Variables x y z : elt.
 
   Property In_dec : reflects (In x s) (mem x s).
@@ -549,15 +524,15 @@ Section InductiveSpec.
     apply is_empty_2; exact H.
     intro abs; rewrite (is_empty_1 abs) in H; discriminate.
   Qed.
-  Corollary is_empty_dec2 : reflects (s [=] empty) (is_empty s).
+  Corollary is_empty_dec2 : reflects (s == empty) (is_empty s).
   Proof.
     destruct is_empty_dec; constructor.
-    intro a; rewrite empty_iff; intuition; contradiction (Htrue a).
+    intro a; rewrite empty_spec; intuition; contradiction (Htrue a).
     intro R; rewrite R in Hfalse; contradiction Hfalse.
     auto with set typeclass_instances.
   Qed.
 
-  Property equal_dec : reflects (s [=] s') (equal s s').
+  Property equal_dec : reflects (s == s') (equal s s').
   Proof.
     case_eq (equal s s'); intro H; constructor.
     apply equal_2; exact H.
@@ -630,3 +605,47 @@ Section InductiveSpec.
     apply max_elt_3; auto.
   Qed.*)
 End InductiveSpec.
+
+Lemma elements_empty `{F : FSet A, @FSetSpecs _ _ _ F} : elements empty = nil.
+Proof.
+assert (Hspec := empty_spec). setoid_rewrite <- elements_spec in Hspec.
+destruct (elements empty) as [| e l]; trivial; [].
+exfalso. rewrite <- (Hspec e). now left.
+Qed.
+
+Lemma cardinal_empty `{F : FSet A, @FSetSpecs _ _ _ F} : cardinal empty = 0.
+Proof. now rewrite cardinal_spec, length_zero_iff_nil, elements_empty. Qed.
+
+Lemma elements_add_incl `{F : FSet A, @FSetSpecs _ _ _ F} :
+  forall x s, inclA equiv (elements (add x s)) (x :: elements s).
+Proof.
+intros x s y. rewrite elements_spec. set_iff. intros [Heq | Hin].
+- now left.
+- right. now rewrite elements_spec.
+Qed.
+
+Lemma elements_add `{F : FSet A, @FSetSpecs _ _ _ F} : forall x s,
+  ~In x s -> PermutationA equiv (elements (add x s)) (x :: elements s).
+Proof.
+intros x s Hx. apply NoDupA_equivlistA_PermutationA.
++ auto with typeclass_instances.
++ apply elements_NoDupA.
++ constructor.
+  - now rewrite elements_spec.
+  - apply elements_NoDupA.
++ intro y. rewrite elements_spec. set_iff.
+  split; intro Hin.
+  - destruct Hin; (now left) || now right; rewrite elements_spec.
+  - inversion_clear Hin; auto; []. right. now rewrite <- elements_spec.
+Qed.
+
+Lemma cardinal_add `{F : FSet A, @FSetSpecs _ _ _ F} : forall x s,
+  ~In x s -> cardinal (add x s) = S (cardinal s).
+Proof. intros. now rewrite 2 cardinal_spec, elements_add. Qed.
+
+Global Instance Set_EqDec elt `{F : FSet elt, @FSetSpecs _ _ _ F} : @EqDec (set elt) _.
+Proof.
+intros s1 s2. destruct (equal s1 s2) eqn:Heq.
+- left. now rewrite <- equal_spec.
+- right. intro Habs. rewrite <- equal_spec, Heq in Habs. discriminate.
+Defined.
